\documentclass{article}
\usepackage[shortlabels]{enumitem}
\usepackage[margin=3cm]{geometry}
\usepackage{amsmath}
\usepackage{amssymb}
\usepackage{graphicx}
\usepackage{listings}
\lstset{
    mathescape=true
}

\title{\Large\bfseries CS 477: Formal Software Development Methods \\
Fall 2016 \\
Homework 1}
\author{Chiao Hsieh, chsieh16@illinois.edu}

\begin{document}
\maketitle

\begin{enumerate}
\item \textbf{[30 points]}
Consider the following program.
\begin{lstlisting}
@pre: $m > 0$
x := 0;
y := 1;
z := 1;
while (x $\neq$ m) {
    z := 2 * z;
    y := y + z;
    x := x + 1;
}
@post: $y = 2^{m + 1} - 1$
\end{lstlisting}

Prove the program satisfies its pre-post condition by giving a proof using
Hoare logic.

You can assume any valid logical statement that is expressed purely in
arithmetic as an axiom

\medskip
Ans.
\medskip

Let loop invariant \verb|@LI:| $0 \leq x \leq m \land z = 2^x \land y = 2^{x + 1} - 1$ ,
we can prove that

Part 1:
\begin{lstlisting}
{$0 \leq x \leq m \land 1 = 2^x \land y = 2^{x + 1} - 1$} z := 1; {@LI} (Axiom)
{$0 \leq x \leq m \land 1 = 2^x \land 1 = 2^{x + 1} - 1$} y := 1; {$0 \leq x \leq m \land 1 = 2^x \land y = 2^{x + 1} - 1$} (Axiom)
{$0 \leq 0 \leq m \land 1 = 2^0 \land 1 = 2^{0 + 1} - 1$} x := 0; {$0 \leq x \leq m \land 1 = 2^x \land 1 = 2^{x + 1} - 1$} (Axiom)
=> {@pre} x := 0 {$0 \leq x \leq m \land 1 = 2^x \land 1 = 2^{x + 1} - 1$} (Consequence)
=> {@pre} x := 0; y := 1; z := 1; {@LI} (Composition)
\end{lstlisting}

Part 2: while loop
\begin{lstlisting}
{$0 \leq (x + 1) \leq m \land z = 2^{(x+1)} \land y = 2^{(x + 1) + 1} - 1$} x := x + 1 {@LI} (Axiom)
{$0 \leq (x + 1) \leq m \land z = 2^{(x+1)} \land y + z = 2^{(x + 1) + 1} - 1$}
    y := y + z;
{$0 \leq (x + 1) \leq m \land z = 2^{(x+1)} \land y = 2^{(x + 1) + 1} - 1$} (Axiom)
{$0 \leq (x + 1) \leq m \land 2*z = 2^{(x+1)} \land y + 2*z = 2^{(x + 1) + 1} - 1$}
    z := 2 * z;
{$0 \leq (x + 1) \leq m \land z = 2^{(x+1)} \land y = 2^{(x + 1) + 1} - 1$} (Axiom)
=> {$0 \leq (x + 1) \leq m \land 2*z = 2^{(x+1)} \land y + 2*z = 2^{(x + 1) + 1} - 1$}
       z := 2 * z; y := y + z; x := x + 1;
   {@LI} (Composition)
=> {$x \neq m\ \land$ @LI} z := 2 * z; y := y + z; x := x + 1; {@LI} (Consequence)
=> {@LI} 
    while (x $\neq$ m) {
       z := 2 * z;
       y := y + z;
       x := x + 1;
    }
    {@LI $\land\ (x = m)$} (Loop)
=>{@LI} 
    while (x $\neq$ m) {
        z := 2 * z;
        y := y + z;
        x := x + 1;
    }
    {@post} (Consequence)
\end{lstlisting}

By applying rule of composition to the 2 parts, we show that the program satisfies pre/post-condition.

\item \textbf{[8*5=40 points]}
For each of the following Hoare triples, write down
\begin{enumerate}[(a)]
\item the weakest pre-condition of the post condition with respect to the program,
\item write down the verification condition using the weakest pre-condition, and
\item formulate the negation of the verification condition in Z3 and report whether it found the verification condition to be valid or not
\end{enumerate}

\medskip
Ans.
\medskip

\begin{enumerate}[(1)]
    \item \verb|{x > 0} y:=x+1; y:=y*2; {y > 0}|

        Weakest Precondition: $(x+1)*2 > 0$ \\
        Verification condition: $x > 0 \implies (x+1)*2 > 0$ \\
        Z3 formula: UNSAT
\begin{verbatim}
(declare-fun x () Int)
(assert (and (> x 0) (not (> (* (+ x 1) 2) 0))))
(check-sat)
\end{verbatim}
        
    \item \verb|{x = y * y} x:=4*x {x > y}|

        Weakest Precondition: $4*x > y$ \\
        Verification condition: $x = y*y \implies 4*x > y$ \\
        Z3 formula: SAT when $x=0 \land y=0$
\begin{verbatim}
(declare-fun x () Int)
(declare-fun y () Int)
(assert (and (= x (* y y)) (not (> (* 4 x) y))))
(check-sat)
\end{verbatim}

\item @pre $\implies$ wp(\verb|x := 0; y := 1; z := 1;|, @LI)

        Weakest Precondition: $0 \leq x \leq m \land 1 = 2^x \land 1 = 2^{x + 1} - 1$ \\
        Verification condition: $m > 0 \implies (0 \leq x \leq m \land 1 = 2^x \land 1 = 2^{0 + 1} - 1)$ \\
        Z3 formula: UNKNOWN
\begin{verbatim}
(declare-const x Int)
(declare-const m Int)

(assert 
(and (> m 0) 
     (not (and (<= 0 x) (<= x m) (= 1 (^ 2 x))
               (= 1 (- (^ 2 (+ 0 1)) 1)))))
)
(check-sat)
\end{verbatim}

\item (@LI $\land\ x \neq m) \implies$ wp(\verb|z := 2 * z; y := y + z; x := x + 1;|, @LI)

        Weakest Precondition: $0 \leq (x + 1) \leq m \land z = 2^x \land y = 2^{x + 1} - 1$ \\
        Verification condition:\\
        $0 \leq x \leq m \land z = 2^x \land y = 2^{x + 1} - 1 \land x \neq m$ \\
        $\implies (0 \leq (x + 1) \leq m \land z = 2^x \land y = 2^{x + 1} - 1)$ \\
        Z3 formula: UNKNOWN
\begin{verbatim}
(declare-const x Int)
(declare-const y Int)
(declare-const z Int)
(declare-const m Int)

(assert 
    (and (and (not (= x m)) (<= 0 x) (<= x m) (= z (^ 2 x))
              (= y (- (^ 2 (+ x 1)) 1)))
         (not (and (<= 0 (+ x 1)) (<= (+ x 1) m) (= (* 2 z) (^ 2 (+ x 1)))
                   (= (+ y (* 2 z)) (- (^ 2 (+ (+ x 1) 1)) 1))
              )
         )
    )
)
(check-sat)
\end{verbatim}

\item @LI $\land\ \neg(x\neq m) \implies$ @post

        Verification condition:\\
        $0 \leq x \leq m \land z = 2^x \land y = 2^{x + 1} - 1 \land \neg(x \neq m) \implies y = 2^{m+1} - 1$\\
        Z3 formula: UNSAT
        
\end{enumerate}

\end{enumerate}

\end{document}